arithmetic up to infinity-norm-exceeds

libcrux-ml-dsa/src/simd/avx2/arithmetic.rs
@@ -150,7 +150,11 @@ pub(super) fn shift_left_then_reduce<const SHIFT_BY: i32>(simd_unit: &mut Vec256
 // additional KATs.
 #[inline(always)]
 #[hax_lib::fstar::before(r#"[@@ "opaque_to_smt"]"#)]
-#[hax_lib::fstar::verification_status(lax)]
+#[hax_lib::requires(fstar!(r#"v $bound > 0 /\ 
+    (forall i. Spec.Utils.is_i32b (v $FIELD_MODULUS - 1) (to_i32x8 ${simd_unit} i))"#))]
+#[hax_lib::ensures(|result| fstar!(r#"
+    $result == false <==> 
+        (forall i. Spec.Utils.is_i32b (v $bound - 1) (to_i32x8 ${simd_unit} i))"#))]
 pub(super) fn infinity_norm_exceeds(simd_unit: &Vec256, bound: i32) -> bool {
     let absolute_values = mm256_abs_epi32(*simd_unit);
 
@@ -162,6 +166,8 @@ pub(super) fn infinity_norm_exceeds(simd_unit: &Vec256, bound: i32) -> bool {
 
     // If every lane of |result| is 0, all coefficients are <= bound - 1
     let result = mm256_testz_si256(compare_with_bound, compare_with_bound);
+
+    hax_lib::fstar!(r"logand_mask_lemma_forall #i32_inttype");
 
     result != 1
 }
